working/composition/event_based_refinement/load_balancer/LoadBalancer.dfy
@@ -1,0 +1,45 @@
+include "AdditionServiceSpec.dfy"
+
+module LoadBalancerHost {
+    import opened Types
+
+    datatype Constants = Constants()
+
+    datatype Variables = Variables(receivedRequest: bool, receivedResponse: bool)
+
+    ghost predicate Init(c: Constants, v: Variables) {
+        && !v.receivedRequest
+        && !v.receivedResponse
+    }
+
+    ghost predicate ForwardRequest(c: Constants, v: Variables, v': Variables, evt: Event, msgOps: MessageOps) {
+        && !v.receivedRequest
+        && v'.receivedRequest
+        && v.receivedResponse == v'.receivedResponse
+        && msgOps.recv.Some?
+        && msgOps.recv.value.ClientRequest?
+        && msgOps.send == Some(LBRequest(msgOps.recv.value.x, msgOps.recv.value.y))
+    }
+
+    ghost predicate ForwardResponse(c: Constants, v: Variables, v': Variables, evt: Event, msgOps: MessageOps) {
+        && !v.receivedResponse
+        && v'.receivedResponse
+        && v.receivedRequest == v'.receivedRequest
+        && msgOps.recv.Some?
+        && msgOps.recv.value.LBResponse?
+        && msgOps.send == Some(ClientResponse(msgOps.recv.value.sum))
+    }
+
+    ghost predicate Next(c: Constants, v: Variables, v': Variables, evt: Event, msgOps: MessageOps)
+    {
+        match evt {
+            case Compute => v == v'
+            case NoOp => 
+            ForwardRequest(c, v, v', evt, msgOps) 
+            || ForwardResponse(c, v, v', evt, msgOps) 
+            || (&& ((msgOps.send.None? || !msgOps.send.value.LBRequest?) && (msgOps.recv.None? || !msgOps.recv.value.ClientRequest?))
+                && ((msgOps.send.None? || !msgOps.send.value.ClientResponse?) && (msgOps.recv.None? || !msgOps.recv.value.LBResponse?))
+                && v == v')
+        }
+    }
+}
