working/composition/event_based_refinement/load_balancer/no_load_balancer/Network.dfy
@@ -1,0 +1,28 @@
+include "AdditionServiceSpec.dfy"
+
+// copied from chapter 5 exercise 1
+module Network {
+  import opened Types
+
+  datatype Constants = Constants  // no constants for network
+
+  // Network state is the set of messages ever sent. Once sent, we'll
+  // allow it to be delivered over and over.
+  // (We don't have packet headers, so duplication, besides being realistic,
+  // also doubles as how multiple parties can hear the message.)
+  datatype Variables = Variables(sentMsgs:set<Message>)
+
+  ghost predicate Init(c: Constants, v: Variables)
+  {
+    && v.sentMsgs == {}
+  }
+
+  ghost predicate Next(c: Constants, v: Variables, v': Variables, msgOps: MessageOps)
+  {
+    // Only allow receipt of a message if we've seen it has been sent.
+    && (msgOps.recv.Some? ==> msgOps.recv.value in v.sentMsgs)
+    // Record the sent message, if there was one.
+    && v'.sentMsgs ==
+      v.sentMsgs + if msgOps.send.None? then {} else { msgOps.send.value }
+  }
+}
